src/Impl_vm.v
@@ -13,35 +13,38 @@ Require Import Maps.
 
 (** Monadic VM implementation *)
 
-Fixpoint copland_compile (t:AnnoTerm): CVM unit :=
+Fixpoint copland_compile (t:AnnoTermPar): CVM unit :=
   match t with
-  | aasp (n,_) a =>
+  | aasp_par (n,_) a =>
       e <- do_prim n a ;;
       put_ev e
-  | aatt (i,j) q t' =>
+  | aatt_par (i,j) q t' =>
       sendReq t' q i ;;
       e' <- receiveResp t' q j ;;
       put_ev e'
-  | alseq _ t1 t2 =>
+  | alseq_par _ t1 t2 =>
       copland_compile t1 ;;
       copland_compile t2
-  | abseq (x,y) sp t1 t2 =>
-      e2 <- split_ev x sp ;;
-      copland_compile t1 ;;
-      e1r <- get_ev ;;
-      put_ev e2 ;;
-      copland_compile t2 ;;
-      e2r <- get_ev ;;
-      join_seq (Nat.pred y) e1r e2r
-  | abpar (x,y) sp t1 t2 =>
-    e2 <- split_ev x sp ;;
+  | abseq_par (x,y) sp t1 t2 =>
+    pr <- split_ev_seq x sp ;;
+    let '(e1,e2) := pr in
+    put_ev e1 ;;
     copland_compile t1 ;;
     e1r <- get_ev ;;
     put_ev e2 ;;
     copland_compile t2 ;;
     e2r <- get_ev ;;
-    join_par (Nat.pred y) e1r e2r
+    join_seq (Nat.pred y) e1r e2r
+  | abpar_par (x,y) loc sp t1 t2 =>
+    pr <- split_ev sp ;;
+    let '(e1,e2) := pr in
+    start_par_thread x loc t2 e2 ;;
+    put_ev e1 ;;
+    copland_compile t1 ;;
+    e1r <- get_ev ;;
+    e2r <- wait_par_thread (Nat.pred y) loc t2 e2 ;;
+    join_par e1r e2r
   end.
 
-Definition run_cvm (t:AnnoTerm) st : cvm_st :=
+Definition run_cvm (t:AnnoTermPar) st : cvm_st :=
   execSt (copland_compile t) st.
