src/StVM.v
@@ -9,12 +9,24 @@ Require Import Maps.
 Require Import List.
 Import ListNotations.
 
+Inductive CVM_Event: Set :=
+| cvm_copy:  nat -> Plc -> CVM_Event 
+| cvm_umeas: nat -> Plc -> ASP_ID -> (list Arg) -> Plc -> TARG_ID -> CVM_Event
+| cvm_sign: nat -> Plc -> Evidence -> CVM_Event
+| cvm_hash: nat -> Plc -> Evidence -> CVM_Event
+| cvm_req: nat -> Plc -> Plc -> Term -> Evidence -> CVM_Event
+| cvm_rpy: nat -> Plc -> Plc -> Evidence -> CVM_Event 
+| cvm_split: nat -> Plc -> CVM_Event
+| cvm_splitp: nat -> Loc -> Plc -> AnnoTerm -> Evidence -> CVM_Event
+| cvm_join:  nat -> Plc -> CVM_Event
+| cvm_joinp:  nat -> Loc -> Plc -> AnnoTerm -> CVM_Event.
+
 (* Specific VM monad state *)
 (*Definition ev_store := MapC nat EvidenceC. *)
 Record cvm_st : Type := mk_st
                           {st_ev:EvC ;
                            (*st_evT: Evidence ; *)
-                           st_trace:list Ev ;
+                           st_trace:list CVM_Event ;
                            st_pl:Plc (*;
                            st_store:ev_store*)}.
 
